add soundness proof from scala-escape

dev2019/stlc1.v
@@ -234,8 +234,8 @@ Hint Resolve ex_intro.
 
 Definition length_env {X : Type} (c : class) (env : env X): nat :=
 match env, c with
-| Def l1 l2 n, First => length l1
-| Def l1 l2 n, Second => length l2
+| Def _ l1 l2 n, First => length l1
+| Def _ l1 l2 n, Second => length l2
 end
 .
 
@@ -256,18 +256,17 @@ Lemma index_max : forall X vs n (T: X),
                        n < length vs.
 Proof.
   intros X vs. induction vs.
-  Case "nil". intros. inversion H.
-  Case "cons".
-  intros. inversion H.
-  case_eq (beq_nat n (length vs)); intros E.
-  SCase "hit".
-  rewrite E in H1. inversion H1. subst.
-  eapply beq_nat_true in E.
-  unfold length. unfold length in E. rewrite E. eauto.
-  SCase "miss".
-  rewrite E in H1.
-  assert (n < length vs). eapply IHvs. apply H1.
-  compute. eauto.
+  - (* nil *) intros. inversion H.
+  - (* case *) intros. inversion H.
+    case_eq (beq_nat n (length vs)); intros E.
+    + (* SCase "hit". *)
+      rewrite E in H1. inversion H1. subst.
+      eapply beq_nat_true in E.
+      unfold length. unfold length in E. rewrite E. eauto.
+    + (* SCase "miss". *)
+      rewrite E in H1.
+      assert (n < length vs). eapply IHvs. apply H1.
+      compute. eauto.
 Qed.
 
 Hint Immediate index_max.
@@ -279,7 +278,344 @@ Proof.
   intros X vs; destruct vs as [l1 l2 n].
   intros x T H.
   destruct x. destruct c; simpl.
-  Case "VFst". inversion H; eauto.
-  Case "VSnd". inversion H.
+  - (* Case "VFst". *) inversion H; eauto.
+  - (* Case "VSnd". *) inversion H.
     destruct (ble_nat n i); inversion H1; eauto.
+Qed.
+
+(* ############################################################ *)
+(*                                                              *)
+(*                 Type soundness for STLC 1/2                  *)
+(*                                                              *)
+(* ############################################################ *)
+
+Require Export SfLib.
+
+Require Export Arith.EqNat.
+Require Export Arith.Le.
+
+Require Export stlc1.
+
+
+(* ############################################################ *)
+(* Definitions                                                  *)
+(* ############################################################ *)
+
+(* ### Value typing and well-typed runtime environments ### *)
+
+Inductive wf_env : venv -> tenv -> Prop := 
+| wfe_nil : forall n, wf_env (Def vl nil nil n) (Def ty nil nil n)
+| wfe_cons : forall v t vs ts n,
+    val_type (expand_env vs v n) v t ->
+    wf_env vs ts ->
+    get_inv_idx vs = get_inv_idx ts ->
+    wf_env (expand_env vs v n) (expand_env ts t n)
+
+with val_type : venv -> vl -> ty -> Prop :=
+| v_bool: forall venv b,
+    val_type venv (vbool b) TBool
+| v_abs: forall env venv tenv y T1 T2 m,
+    wf_env venv tenv ->
+    has_type (expand_env (expand_env tenv (TFun T1 m T2) Second) T1 m) y First T2 ->
+    val_type env (vabs venv m y) (TFun T1 m T2)
+.
+
+
+(* type equivalence: only via reflexivity *)
+Inductive stp: venv -> ty -> venv -> ty -> Prop :=
+| stp_refl: forall G1 G2 T,
+   stp G1 T G2 T.
+
+Hint Constructors val_type.
+Hint Constructors wf_env.
+
+Hint Unfold expand_env.
+
+Lemma length_env_incr : forall (X : Type) n m env (x : X),
+   n = m ->
+   length_env n (expand_env env x m) = 1 + length_env n env.
+Proof.
+  intros. destruct env; destruct n; inversion H; auto.
+Qed.
+   
+Lemma length_env_same : forall (X : Type) n m env (x : X),
+   n <> m ->
+   length_env n (expand_env env x m) = length_env n env.
+Proof.
+  intros. destruct env; destruct n; destruct m.
+      apply ex_falso_quodlibet; auto.
+      auto.
+      auto.
+      apply ex_falso_quodlibet; auto.
+Qed.
+
+Hint Rewrite length_env_incr.
+Hint Rewrite length_env_same.
+Hint Unfold not.
+
+Lemma wf_length : forall vs ts,
+      wf_env vs ts ->
+      length_env First vs = length_env First ts /\ length_env Second vs = length_env Second ts.
+Proof.
+  intros. induction H; auto.
+  destruct IHwf_env as [L R].
+  destruct n. 
+  Case "First"; split.
+  repeat rewrite length_env_incr; auto.
+  repeat rewrite length_env_same; auto.
+  unfold not; intros. inversion H2. unfold not; intros. inversion H2.
+  Case "Second"; split.
+  repeat rewrite length_env_same; auto.
+  unfold not; intros. inversion H2. unfold not; intros. inversion H2.
+  repeat rewrite length_env_incr; auto.
+Qed.
+
+Hint Immediate wf_length.
+
+
+
+Lemma wf_idx : forall vs ts,
+      wf_env vs ts ->
+      get_inv_idx vs = get_inv_idx ts.
+Proof.
+  intros. induction H; auto.
+  destruct vs; destruct ts; destruct n; auto.
+Qed.
+
+Hint Immediate wf_idx.
+
+
+Lemma valtp_extend : forall vs v v1 T n,
+                       val_type vs v T ->
+                       val_type (expand_env vs v1 n) v T.
+Proof. intros. induction H; eauto. Qed.
+
+Lemma index_extend : forall X vs n a (T: X),
+                       index n vs = Some T ->
+                       index n (a::vs) = Some T.
+
+Proof.
+  intros.
+  assert (n < length vs). eapply index_max. eauto.
+  assert (n <> length vs). omega.
+  assert (beq_nat n (length vs) = false) as E. eapply beq_nat_false_iff; eauto.
+  unfold index. unfold index in H. rewrite H. rewrite E. reflexivity.
+Qed.
+
+Hint Immediate index_extend.
+
+Lemma lookup_extend : forall X vs x a (T: X) n,
+                       lookup x vs = Some T ->
+                       lookup x (expand_env vs a n) = Some T.
+
+Proof.
+  intros.
+  assert (get_idx x < length_env (get_class x) vs). eapply lookup_max. eauto.
+  assert (get_idx x <> length_env (get_class x) vs). omega.
+  assert (beq_nat (get_idx x) (length_env (get_class x) vs) = false) as E. eapply beq_nat_false_iff; eauto.
+  destruct vs.
+  destruct n; destruct x; destruct c; simpl in E;
+    inversion H; simpl; try rewrite E; auto.
+Qed.
+
+(*
+Lemma index_safe_ex: forall Hl1 Hl2 Gl1 Gl2 Hidx Gidx TF i,
+   wf_env (Def vl Hl1 Hl2 Hidx) (Def ty Gl1 Gl2 Gidx) ->
+   index i Gl1 = Some TF ->
+   exists v, index i Hl1 = Some v.
+Proof. intros.
+  apply wf_length in H. destruct H as [L _]. simpl in L.
+  
+Qed.
+*)
+
+Lemma lookup_safe_ex: forall H1 G1 TF x,
+             wf_env H1 G1 ->
+             lookup x G1 = Some TF ->
+             exists v, lookup x H1 = Some v /\ val_type H1 v TF.
+Proof. intros. induction H.
+  Case "nil". inversion H0. destruct x; destruct c; destruct (ble_nat n i); inversion H1.
+  Case "cons". destruct vs as [vl1 vl2 vidx]. destruct ts as [tl1 tl2 tidx].
+    apply wf_length in H1. destruct H1 as [H1l H1r].
+    destruct x; destruct c; inversion H0.
+    SCase "VFst". destruct n; simpl in H0 ; simpl in H2.
+      SSCase "First".
+        case_eq (beq_nat i (length tl1)).
+        SSSCase "hit".
+          intros E.
+          rewrite E in H0. inversion H0. subst t. simpl.
+          assert (beq_nat i (length vl1) = true). eauto.
+          rewrite H1. eauto.
+        SSSCase "miss".
+          intros E.
+          assert (beq_nat i (length vl1) = false). eauto.
+          assert (exists v0, lookup (V First i) (Def vl vl1 vl2 vidx) = Some v0 /\ val_type (Def vl vl1 vl2 vidx) v0 TF) as HI.
+          eapply IHwf_env. simpl. rewrite E in H0. eauto.
+          inversion HI as [v0 HI1]. inversion HI1.
+          eexists. econstructor. eapply lookup_extend; eauto. eapply valtp_extend; eauto.
+     SSCase "Second".
+       assert (exists v0, lookup (V First i) (Def vl vl1 vl2 vidx) = Some v0 /\ val_type (Def vl vl1 vl2 vidx) v0 TF) as HI.
+       eapply IHwf_env. simpl. eauto.
+       inversion HI as [v0 HI1]. inversion HI1.
+       eexists. econstructor. eapply lookup_extend; eauto. eapply valtp_extend; eauto.
+   SCase "VSnd". destruct n; simpl in H0; simpl in H2.
+     SSCase "First".
+       assert (exists v0, lookup (V Second i) (Def vl vl1 vl2 vidx) = Some v0 /\ val_type (Def vl vl1 vl2 vidx) v0 TF) as HI.
+       eapply IHwf_env. simpl. eauto.
+       inversion HI as [v0 HI1]. inversion HI1.
+       eexists. econstructor. eapply lookup_extend; eauto. eapply valtp_extend; eauto.
+     SSCase "Second".
+       case_eq (beq_nat i (length tl2)).
+        SSSCase "hit".
+          intro E.
+          rewrite E in H0. simpl. destruct (ble_nat tidx i); inversion H0.
+          subst t.
+          assert (beq_nat i (length vl2) = true). eauto.
+          rewrite H1. inversion H3. subst vidx. destruct (ble_nat tidx i); eauto. inversion H5.
+        SSSCase "miss".
+          intro E.
+          assert (beq_nat i (length vl2) = false). eauto.
+          assert (exists v0, lookup (V Second i) (Def vl vl1 vl2 vidx) = Some v0 /\ val_type (Def vl vl1 vl2 vidx) v0 TF) as HI.
+          eapply IHwf_env. simpl. destruct (ble_nat tidx i). inversion H0. rewrite E in H0. rewrite H0. rewrite E. auto. auto.
+          inversion HI as [v0 HI1]. inversion HI1.
+          eexists. econstructor. eapply lookup_extend; eauto. eapply valtp_extend; eauto.
+Qed.
+  
+Inductive res_type: venv -> option vl -> ty -> Prop :=
+| not_stuck: forall venv v T,
+      val_type venv v T ->
+      res_type venv (Some v) T.
+
+Hint Constructors res_type.
+Hint Resolve not_stuck.
+
+
+Lemma valtp_widen: forall vf H1 H2 T1 T2,
+  val_type H1 vf T1 ->
+  stp H1 T1 H2 T2 ->
+  val_type H2 vf T2.
+Proof.
+  intros. inversion H; inversion H0; subst T2; subst; eauto.
+Qed.
+
+Lemma invert_abs: forall venv vf vx T1 n T2,
+  val_type venv vf (TFun T1 n T2) ->
+  exists env tenv y T3 T4,
+    vf = (vabs env n y) /\
+    wf_env env tenv /\
+    has_type (expand_env (expand_env tenv (TFun T3 n T4) Second) T3 n) y First T4 /\
+    stp venv T1 (expand_env (expand_env env vf Second) vx n) T3 /\
+    stp (expand_env (expand_env env vf Second) vx n) T4 venv T2.
+Proof.
+  intros. inversion H. repeat eexists; repeat eauto.
+Qed.
+
+
+Lemma ext_sanitize_commute : forall {T} n venv (v:T) c,
+   expand_env (sanitize_any venv n) v c = sanitize_any (expand_env venv v c) n.
+Proof.
+  intros. destruct venv. destruct c; simpl; eauto. 
+Qed.
+
+Lemma val_type_sanitize_any : forall n venv res T,
+  val_type venv res T ->
+  val_type (sanitize_any venv n) res T.
+Proof.
+  intros. inversion H; eauto.
+Qed.
+
+Lemma val_type_sanitize : forall env res T n,
+  val_type (sanitize_env n env) res T ->
+  val_type env res T.
+Proof.
+  intros. inversion H; eauto.
+Qed.
+
+Lemma wf_sanitize_any : forall n venv tenv,
+   wf_env venv tenv ->
+   wf_env (sanitize_any venv n) (sanitize_any tenv n).
+Proof.
+  intros. induction H.
+  - simpl. eapply wfe_nil.
+  - eapply wfe_cons in IHwf_env.
+    rewrite <-ext_sanitize_commute. rewrite <-ext_sanitize_commute.
+    eauto. eauto. rewrite ext_sanitize_commute.
+    eapply val_type_sanitize_any in H. eauto. eauto.
+Qed.  
+
+Lemma wf_sanitize : forall n venv tenv,
+   wf_env venv tenv ->
+   wf_env (sanitize_env n venv) (sanitize_env n tenv).
+Proof.
+  intros. destruct n; unfold sanitize_env. destruct venv. destruct tenv.
+  assert (length l0 = length l2). apply wf_length in H; destruct H as [L R]; eauto.
+  rewrite H0. eapply wf_sanitize_any. eauto.
+  eauto.
+Qed.
+  
+
+Hint Immediate wf_sanitize.
+   
+
+(* ### Theorem 3.5 ### *)
+(* if result of STLC 1/2 evaluation is not a timeout, then *)
+(* it is not stuck, and well-typed *)
+
+Theorem full_safety : forall k e n tenv venv res T,
+  teval k venv e n = Some res -> has_type tenv e n T -> wf_env venv tenv ->
+  res_type venv res T.
+
+Proof.
+  intros k. induction k.
+  (* 0 *)   intros. inversion H.
+  (* S n *) intros. destruct e; inversion H; inversion H0. 
+  
+  - Case "True".  eapply not_stuck. eapply v_bool.
+  - Case "False". eapply not_stuck. eapply v_bool.
+
+  - Case "Var".
+    subst.
+    destruct (lookup_safe_ex (sanitize_env n venv) (sanitize_env n tenv) T v) as [va [I V]]; eauto. 
+
+    rewrite I. eapply not_stuck. eapply val_type_sanitize. eapply V.
+
+  - Case "App".
+    remember (teval k venv e1 Second) as tf.
+    subst T. subst n0.
+    
+    destruct tf as [rf|]; try solve by inversion.
+    assert (res_type venv rf (TFun T1 m T2)) as HRF. SCase "HRF". subst. eapply IHk; eauto.
+    inversion HRF as [? vf].
+
+    subst rf. remember vf as rvf. destruct vf; try (subst rvf; solve by inversion).
+    assert (c = m). destruct m; destruct c; try (subst rvf ; solve by inversion); eauto. subst c. subst rvf.
+    remember (teval k venv e2 m) as tx.
+
+    destruct tx as [rx|]; try solve by inversion.
+    assert (res_type venv rx T1) as HRX. SCase "HRX". subst. eapply IHk; eauto.
+    inversion HRX as [? vx]. 
+
+    destruct (invert_abs venv (vabs e m t) vx T1 m T2) as
+        [env1 [tenv1 [y0 [T3 [T4 [EF [WF [HTY [STX STY]]]]]]]]]. eauto.
+    (* now we know it's a closure, and we have has_type evidence *)
+
+    inversion EF. subst e. subst y0. clear EF.
+    subst rx.
+
+    assert (res_type (expand_env (expand_env env1 (vabs env1 m t) Second) vx m) res T4) as HRY.
+        SSSCase "HRY".
+          subst. eapply IHk; eauto.
+        (* wf_env f x *) econstructor. eapply valtp_widen; eauto.
+        (* wf_env f   *) econstructor. eapply v_abs; eauto.
+          eauto.
+          apply wf_idx. assumption.
+          apply wf_idx. econstructor. eauto. assumption. apply wf_idx. assumption.
+
+    inversion HRY as [? vy].
+
+    eapply not_stuck. eapply valtp_widen; eauto.
+    
+  - Case "Abs". intros. inversion H. inversion H0.
+    eapply not_stuck. eapply v_abs; eauto.
+    eauto.
 Qed.
